Fixing Simpl/Complx refinement proofs for Set and List
Signed-off-by: Roni Häcki <roni.haecki@inf.ethz.ch>

CleanQ/CleanQ_SetListRefinement.thy
@@ -19,15 +19,75 @@ theory CleanQ_SetListRefinement imports
 begin
 
 
+(* ==================================================================================== *)
+subsection \<open>Set Pre- and post- conditions\<close>
+(* ==================================================================================== *)
+
+definition CleanQ_Set_deq_x_pre :: 
+  "'a set \<Rightarrow> 'a \<Rightarrow> ('a CleanQ_Set_State, 'a CleanQ_Set_State) Semantic.xstate set"
+  where "CleanQ_Set_deq_x_pre K b = Semantic.Normal ` { rb. I1 rb K \<and> I2 rb \<and> b \<in> TYX rb }"
+
+definition CleanQ_Set_deq_x_post :: 
+  "'a set \<Rightarrow> 'a \<Rightarrow> ('a CleanQ_Set_State, 'a CleanQ_Set_State) Semantic.xstate set"
+  where "CleanQ_Set_deq_x_post K b = Semantic.Normal ` { rb. I1 rb K \<and> I2 rb \<and> b \<in> SX rb }"
+
+definition CleanQ_Set_deq_y_pre :: 
+  "'a set \<Rightarrow> 'a \<Rightarrow> ('a CleanQ_Set_State, 'a CleanQ_Set_State) Semantic.xstate set"
+  where "CleanQ_Set_deq_y_pre K b = Semantic.Normal ` { rb. I1 rb K \<and> I2 rb \<and> b \<in> TXY rb }"
+
+definition CleanQ_Set_deq_y_post :: 
+  "'a set \<Rightarrow> 'a \<Rightarrow> ('a CleanQ_Set_State, 'a CleanQ_Set_State) Semantic.xstate set"
+  where "CleanQ_Set_deq_y_post K b = Semantic.Normal ` { rb. I1 rb K \<and> I2 rb \<and> b \<in> SY rb }"
+
+
+definition CleanQ_Set_enq_x_pre :: 
+  "'a set \<Rightarrow> 'a \<Rightarrow> ('a CleanQ_Set_State, 'a CleanQ_Set_State) Semantic.xstate set"
+  where "CleanQ_Set_enq_x_pre K b = Semantic.Normal ` { rb. I1 rb K \<and> I2 rb \<and> b \<in> SX rb }"
+
+definition CleanQ_Set_enq_x_post :: 
+  "'a set \<Rightarrow> 'a \<Rightarrow> ('a CleanQ_Set_State, 'a CleanQ_Set_State) Semantic.xstate set"
+  where "CleanQ_Set_enq_x_post K b = Semantic.Normal ` { rb. I1 rb K \<and> I2 rb \<and> b \<in> TXY rb }"
+
+definition CleanQ_Set_enq_y_pre :: 
+  "'a set \<Rightarrow> 'a \<Rightarrow> ('a CleanQ_Set_State, 'a CleanQ_Set_State) Semantic.xstate set"
+  where "CleanQ_Set_enq_y_pre K b = Semantic.Normal ` { rb. I1 rb K \<and> I2 rb \<and> b \<in> SY rb }"
+
+definition CleanQ_Set_enq_y_post :: 
+  "'a set \<Rightarrow> 'a \<Rightarrow> ('a CleanQ_Set_State, 'a CleanQ_Set_State) Semantic.xstate set"
+  where "CleanQ_Set_enq_y_post K b = Semantic.Normal ` { rb. I1 rb K \<and> I2 rb \<and> b \<in> TYX rb }"
+
+
+(* ==================================================================================== *)
+subsection \<open>List Pre- conditions\<close>
+(* ==================================================================================== *)
+
+definition CleanQ_List_enq_x_pre :: "'a set \<Rightarrow> 'a \<Rightarrow> ('a CleanQ_List_State, 'a CleanQ_List_State) Semantic.xstate set"
+  where "CleanQ_List_enq_x_pre K b =  Semantic.Normal ` {rb. CleanQ_List_Invariants K rb \<and> b \<in> lSX rb \<and> b \<notin> set (lTXY rb)}"
+
+definition CleanQ_List_enq_y_pre :: "'a set \<Rightarrow> 'a \<Rightarrow> ('a CleanQ_List_State, 'a CleanQ_List_State) Semantic.xstate set"
+  where "CleanQ_List_enq_y_pre K b = Semantic.Normal ` {rb. CleanQ_List_Invariants K rb \<and> b \<in> lSY rb \<and> b \<notin> set (lTYX rb)}"
+
+definition CleanQ_List_deq_x_pre :: "'a set \<Rightarrow> 'a \<Rightarrow> ('a CleanQ_List_State, 'a CleanQ_List_State) Semantic.xstate set"        
+  where "CleanQ_List_deq_x_pre K buf = Semantic.Normal ` {rb.  CleanQ_List_Invariants K rb \<and>
+                                                          (lTYX rb) \<noteq> [] \<and> buf = hd (lTYX rb) }"
+
+definition CleanQ_List_deq_y_pre :: "'a set \<Rightarrow> 'a \<Rightarrow> ('a CleanQ_List_State, 'a CleanQ_List_State) Semantic.xstate set"        
+  where "CleanQ_List_deq_y_pre K buf = Semantic.Normal ` {rb. CleanQ_List_Invariants K rb \<and>
+                                                          (lTXY rb) \<noteq> [] \<and> buf = hd (lTXY rb) }"
+(* ==================================================================================== *)
+subsection \<open>Refinement\<close>
+(* ==================================================================================== *)
+
 
 lemma
   CleanQ_setListRefinement_enq_x: "((\<Gamma>a, CleanQ_Set_enq_x_pre K buf, Language.Basic (CleanQ_Set_enq_x buf)), 
                                (\<Gamma>c, CleanQ_List_enq_x_pre K buf, Language.Basic (CleanQ_List_enq_x buf)))
                                \<in> refinement_s (separable_lift CleanQ_List2Set CleanQ_List2Set)"
 apply(rule refinement_s_BasicI) (* Problem applying this after unfolding*)
-  unfolding separable_lift_def CleanQ_List2Set_def CleanQ_Set_enq_x_def CleanQ_Set_enq_x_pre_def CleanQ_List_enq_x_def
-  CleanQ_List_enq_x_pre_def
-  by(auto)
+  unfolding separable_lift_def CleanQ_List2Set_def CleanQ_List_enq_x_def CleanQ_Set_enq_x_def 
+  CleanQ_List_enq_x_pre_def CleanQ_Set_enq_x_pre_def 
+   apply auto
+  by (simp add: CleanQ_List2Set_def CleanQ_List_Invariants_def I1_list_img_lift I2_list_img_lift)
 
 lemma
   CleanQ_setListRefinement_enq_y: "((\<Gamma>a, CleanQ_Set_enq_y_pre K buf, Language.Basic (CleanQ_Set_enq_y buf)), 
@@ -36,20 +96,21 @@ lemma
   apply(rule refinement_s_BasicI) (* Problem applying this after unfolding*)
    unfolding separable_lift_def CleanQ_List2Set_def  CleanQ_Set_enq_y_def CleanQ_Set_enq_y_pre_def CleanQ_List_enq_y_def
   CleanQ_List_enq_y_pre_def
-  by(auto)
+   apply(auto)
+   by (simp add: CleanQ_List2Set_def CleanQ_List_Invariants_def I1_list_img_lift I2_list_img_lift)
 
 lemma
   CleanQ_setListRefinement_deq_x: "((\<Gamma>a, CleanQ_Set_deq_x_pre K buf, Language.Basic (CleanQ_Set_deq_x buf)), 
                                (\<Gamma>c, CleanQ_List_deq_x_pre K buf, Language.Basic (CleanQ_List_deq_x)))
                                \<in> refinement_s (separable_lift CleanQ_List2Set CleanQ_List2Set)"
   apply(rule refinement_s_BasicI) (* Problem applying this after unfolding*)
-    unfolding separable_lift_def  CleanQ_Set_deq_x_def CleanQ_Set_deq_x_pre_def CleanQ_List_deq_x_def
-   CleanQ_List_deq_x_pre_def
-   apply(auto)
- unfolding CleanQ_List2Set_def  
-   apply(simp add:list_set_hd_tl_subtract)
-  by(auto)
-  
+  unfolding separable_lift_def  CleanQ_Set_deq_x_def CleanQ_Set_deq_x_pre_def CleanQ_List_deq_x_def
+   CleanQ_List_deq_x_pre_def CleanQ_List_Invariants_def CleanQ_List2Set_def
+  apply auto
+  apply (simp add: list.set_sel(2))
+  apply (metis I3_def distinct.simps(2) hd_Cons_tl)
+  using hd_Cons_tl apply force
+  by (simp add: CleanQ_List2Set_def I1_list_img_lift I2_list_img_lift)
 
 lemma
   CleanQ_setListRefinement_deq_y: "((\<Gamma>a, CleanQ_Set_deq_y_pre K buf, Language.Basic (CleanQ_Set_deq_y buf)), 
@@ -57,10 +118,11 @@ lemma
                                \<in> refinement_s (separable_lift CleanQ_List2Set CleanQ_List2Set)"
 apply(rule refinement_s_BasicI) (* Problem applying this after unfolding*)
   unfolding separable_lift_def  CleanQ_Set_deq_y_def CleanQ_Set_deq_y_pre_def CleanQ_List_deq_y_def
-  CleanQ_List_deq_y_pre_def
-   apply(auto)
-  unfolding CleanQ_List2Set_def
-   apply(simp add:list_set_hd_tl_subtract)
-  by(auto)
+  CleanQ_List_deq_y_pre_def CleanQ_List_Invariants_def CleanQ_List2Set_def
+  apply auto
+  apply (simp add: list.set_sel(2))
+  apply (metis I3_def distinct.simps(2) hd_Cons_tl)
+  using hd_Cons_tl apply force
+  by (simp add: CleanQ_List2Set_def I1_list_img_lift I2_list_img_lift)
   
 end
